Continue proofs, reorganise code/fallback

code/fallback/Hacl.IntTypes.Intrinsics.fst
@@ -25,15 +25,40 @@ let add_carry_st (t:inttype{t = U32 \/ t = U64}) =
     (let r = Seq.index (as_seq h1 r) 0 in
     v r + v c * pow2 (bits t) == v x + v y + v cin))
 
+inline_for_extraction noextract
+val cast_to : t:inttype{t = U32 \/ t = U64} ->
+  t':inttype{if t = U32 then t' = U64 else t' = U128} ->
+  (u1:int_t t SEC{unsigned t' \/ range (v u1) t'}
+  -> u2:int_t t' SEC{v u2 == v u1 @%. t'})
+let cast_to t t' =
+  match t with
+  | U32 -> cast U64 SEC
+  | U64 -> cast U128 SEC
 
 inline_for_extraction noextract
-val add_carry_u64: add_carry_st U64
-let add_carry_u64 cin x y r =
-  let res = to_u128 x +. to_u128 cin +. to_u128 y in
-  let c = to_u64 (res >>. 64ul) in
-  r.(0ul) <- to_u64 res;
+val cast_from : t:inttype{t = U64 \/ t = U128} ->
+  t':inttype{if t = U64 then t' = U32 else t' = U64} ->
+  (u1:int_t t SEC{unsigned t' \/ range (v u1) t'}
+  -> u2:int_t t' SEC{v u2 == v u1 @%. t'})
+let cast_from t t' =
+  match t with
+  | U64 -> cast U32 SEC
+  | U128 -> cast U64 SEC
+
+inline_for_extraction noextract
+val add_carry:
+  t:inttype{t = U32 \/ t = U64} ->
+  t':inttype{if t = U32 then t' = U64 else t' = U128} ->
+  shift_bits:UInt32.t{if t = U32 then shift_bits == 32ul else shift_bits == 64ul} ->
+  add_carry_st t
+let add_carry t t' shift_bits cin x y r =
+  let res = cast_to t t' x +. cast_to t t' cin +. cast_to t t'  y in
+  let c = cast_from t' t (res >>. shift_bits) in
+  r.(0ul) <- cast_from t' t res;
   c
 
+val add_carry_u32: add_carry_st U32
+let add_carry_u32 = add_carry U32 U64 32ul
 
 inline_for_extraction noextract
 let sub_borrow_st (t:inttype{t = U32 \/ t = U64}) =
@@ -48,33 +73,33 @@ let sub_borrow_st (t:inttype{t = U32 \/ t = U64}) =
     (let r = Seq.index (as_seq h1 r) 0 in
     v r - v c * pow2 (bits t) == v x - v y - v cin))
 
+val sub_borrow_u32: sub_borrow_st U32
+let sub_borrow_u32 cin x y r =
+  let res = to_u64 x -. to_u64 y -. to_u64 cin in
+  assert (v res == ((v x - v y) % pow2 64 - v cin) % pow2 64);
+  Math.Lemmas.lemma_mod_add_distr (- v cin) (v x - v y) (pow2 64);
+  assert (v res == (v x - v y - v cin) % pow2 64);
 
-inline_for_extraction noextract
-val sub_borrow_u64: sub_borrow_st U64
-let sub_borrow_u64 cin x y r =
-  let res = to_u128 x -. to_u128 y -. to_u128 cin in
-  assert (v res == ((v x - v y) % pow2 128 - v cin) % pow2 128);
-  Math.Lemmas.lemma_mod_add_distr (- v cin) (v x - v y) (pow2 128);
-  assert (v res == (v x - v y - v cin) % pow2 128);
+  assert (v res % pow2 32 = (v x - v y - v cin) % pow2 64 % pow2 32);
+  Math.Lemmas.pow2_modulo_modulo_lemma_1 (v x - v y - v cin) 32 64;
+  assert (v res % pow2 32 = (v x - v y - v cin) % pow2 32);
 
-  assert (v res % pow2 64 = (v x - v y - v cin) % pow2 128 % pow2 64);
-  Math.Lemmas.pow2_modulo_modulo_lemma_1 (v x - v y - v cin) 64 128;
-  assert (v res % pow2 64 = (v x - v y - v cin) % pow2 64);
-
-  let c = to_u64 (res >>. 64ul) &. u64 1 in
+  let c = to_u32 (res >>. 32ul) &. u32 1 in
   assert_norm (pow2 1 = 2);
-  mod_mask_lemma (to_u64 (res >>. 64ul)) 1ul;
-  assert (v ((mk_int #U64 #SEC 1 <<. 1ul) -! mk_int 1) == 1);
-  assert (v c = v res / pow2 64 % pow2 1);
+  mod_mask_lemma (to_u32 (res >>. 32ul)) 1ul;
+  assert (v ((mk_int #U32 #SEC 1 <<. 1ul) -! mk_int 1) == 1);
+  assert (v c = v res / pow2 32 % pow2 1);
 
-  r.(0ul) <- to_u64 res;
+  r.(0ul) <- to_u32 res;
   assert (v c = (if 0 <= v x - v y - v cin then 0 else 1));
   c
 
 
+(* Fallback versions of add_carry_u64 and sub_borrow_u64 for platforms which
+   don't support uint128 *)
 inline_for_extraction noextract
-val add_carry: #t:inttype{t = U32 \/ t = U64} -> add_carry_st t
-let add_carry #t cin x y r =
+val add_carry_fallback: #t:inttype{t = U32 \/ t = U64} -> add_carry_st t
+let add_carry_fallback #t cin x y r =
   let res = x +. cin +. y in
   let c = logand (logor (lt_mask res x) (logand (eq_mask res x) cin)) (uint #t 1) in
   r.(0ul) <- res;
@@ -83,14 +108,12 @@ let add_carry #t cin x y r =
   logand_mask (logor (lt_mask res x) (logand (eq_mask res x) cin)) (uint #t 1) 1;
   c
 
-
-val add_carry_u32: add_carry_st U32
-let add_carry_u32 cin x y r = add_carry #U32 cin x y r
-
+val add_carry_u64_fallback: add_carry_st U64
+let add_carry_u64_fallback cin x y r = add_carry_fallback #U64 cin x y r
 
 inline_for_extraction noextract
-val sub_borrow: #t:inttype{t = U32 \/ t = U64} -> sub_borrow_st t
-let sub_borrow #t cin x y r =
+val sub_borrow_fallback: #t:inttype{t = U32 \/ t = U64} -> sub_borrow_st t
+let sub_borrow_fallback #t cin x y r =
   let res = x -. y -. cin in
   let c = logand (logor (gt_mask res x) (logand (eq_mask res x) cin)) (uint #t 1) in
   logand_lemma (eq_mask res x) cin;
@@ -99,6 +122,5 @@ let sub_borrow #t cin x y r =
   r.(0ul) <- res;
   c
 
-
-val sub_borrow_u32: sub_borrow_st U32
-let sub_borrow_u32 cin x y r = sub_borrow #U32 cin x y r
+val sub_borrow_u64_fallback: sub_borrow_st U64
+let sub_borrow_u64_fallback cin x y r = sub_borrow_fallback #U64 cin x y r
